messageInvariantPrototypes/shardedKv/distributed/applicationProof.dfy
@@ -1,0 +1,160 @@
+// User level proofs of application invariants
+
+include "spec.dfy"
+
+module ShardedKVProof {
+  import opened Types
+  import opened UtilitiesLibrary
+  import opened DistributedSystem
+  import opened Obligations
+
+  ghost predicate KeyInFlight(c: Constants, v: Variables, msg: Message, k: Key) 
+    requires v.WF(c)
+  {
+      && msg in v.network.sentMsgs
+      && c.ValidIdx(msg.dst)
+      && msg.key.key == k
+      && (v.hosts[msg.dst].HasKey(k) ==> msg.key.version > v.hosts[msg.dst].myKeys[k])
+  }
+
+  ghost predicate AtMostOneInFlight(c: Constants, v: Variables)
+    requires v.WF(c)
+  {
+    forall m1, m2, k | 
+      && KeyInFlight(c, v, m1, k) && KeyInFlight(c, v, m2, k) 
+    ::
+      m1 == m2
+  }
+
+  ghost predicate NoneHasKey(c: Constants, v: Variables, k: Key) 
+    requires v.WF(c)
+  {
+    forall idx | c.ValidIdx(idx) :: !v.hosts[idx].HasKey(k)
+  }
+  
+
+  ghost predicate HasKeyImpliesNoneInFlight(c: Constants, v: Variables)
+    requires v.WF(c)
+  {
+    forall k, msg | !NoneHasKey(c, v, k) && msg in v.network.sentMsgs
+    ::
+    !KeyInFlight(c, v, msg, k)
+  }
+
+  
+  ghost predicate ApplicationInv(c: Constants, v: Variables)
+    requires v.WF(c)
+  {
+    && AtMostOneInFlight(c, v)
+    && HasKeyImpliesNoneInFlight(c, v)
+  }
+
+  ghost predicate Inv(c: Constants, v: Variables)
+  {
+    && v.WF(c)
+    && ApplicationInv(c, v)
+    && Safety(c, v)
+  }
+
+  lemma InvImpliesSafety(c: Constants, v: Variables)
+    requires Inv(c, v)
+    ensures Safety(c, v)
+  {}
+
+  lemma InitImpliesInv(c: Constants, v: Variables)
+    requires Init(c, v)
+    ensures Inv(c, v)
+  {}
+
+  lemma InvInductive(c: Constants, v: Variables, v': Variables)
+    requires Inv(c, v)
+    requires Next(c, v, v')
+    ensures Inv(c, v')
+  {
+    assert v'.WF(c);
+    InvNextAtMostOneInFlight(c, v, v');
+    assert AtMostOneInFlight(c, v');
+
+    assume false;
+    assert HasKeyImpliesNoneInFlight(c, v');
+    assert Safety(c, v');
+  }
+
+
+/***************************************************************************************
+*                                 InvNext Proofs                                       *
+***************************************************************************************/
+
+lemma InvNextAtMostOneInFlight(c: Constants, v: Variables, v': Variables)
+  requires v'.WF(c)
+  requires Inv(c, v)
+  requires Next(c, v, v')
+  ensures AtMostOneInFlight(c, v')
+{
+  forall m1, m2, k | 
+    && KeyInFlight(c, v', m1, k) && KeyInFlight(c, v', m2, k) 
+  ensures
+    m1 == m2
+  {
+    assume false;
+  }
+}
+
+lemma InvNextHasKeyImpliesNoneInFlight(c: Constants, v: Variables, v': Variables)
+  requires v'.WF(c)
+  requires Inv(c, v)
+  requires Next(c, v, v')
+  ensures HasKeyImpliesNoneInFlight(c, v')
+{
+  assume false;
+}
+
+lemma InvNextSafety(c: Constants, v: Variables, v': Variables)
+  requires v'.WF(c)
+  requires Inv(c, v)
+  requires Next(c, v, v')
+  ensures Safety(c, v')
+{
+  forall idx1, idx2, k: Key | 
+    && c.ValidIdx(idx1) 
+    && c.ValidIdx(idx2) 
+    && v'.hosts[idx1].HasKey(k)
+    && v'.hosts[idx2].HasKey(k)
+  ensures
+     idx1 == idx2
+  {
+    if idx1 != idx2 {
+      if v.hosts[idx1].HasKey(k) {
+        AtMostOneHostHasKey(c, v, v', k, idx1, idx2);
+      } else if v.hosts[idx2].HasKey(k) {
+        AtMostOneHostHasKey(c, v, v', k, idx2, idx1);
+      }
+    }
+  }
+}
+
+lemma AtMostOneHostHasKey(c: Constants, v: Variables, v': Variables, k: Key, idx: HostId, other: HostId)
+  requires v.WF(c) && v'.WF(c)
+  requires Inv(c, v)
+  requires c.ValidIdx(idx)
+  requires c.ValidIdx(other)
+  requires idx != other
+  requires v.hosts[idx].HasKey(k)
+  requires !v.hosts[other].HasKey(k)
+  requires Next(c, v, v')
+  ensures !v'.hosts[other].HasKey(k)
+{
+  var dsStep :| NextStep(c, v, v', dsStep);
+  var actor, msgOps := dsStep.actor, dsStep.msgOps;
+  if actor == other {
+    var cs, s, s' := c.hosts[other], v.hosts[other], v'.hosts[other];
+    var step :| Host.NextStep(cs, s, s', step, msgOps);
+    if step.ReceiveStep? && v'.hosts[other].HasKey(k) {
+      assert KeyInFlight(c, v, msgOps.recv.value, k);  // trigger
+      assert false;
+    }    
+  }
+}
+
+
+} // end module ShardedKVProof
